@prefix ac:      <#> .
@prefix dcterms:  <http://purl.org/dc/terms/> .
@prefix event:   <http://purl.org/NET/c4dm/event.owl#> .
@prefix foaf:    <http://xmlns.com/foaf/0.1/> .
@prefix frbr:    <http://purl.org/vocab/frbr/core#> .
@prefix mo:      <http://purl.org/ontology/mo/> .
@prefix owl:     <http://www.w3.org/2002/07/owl#> .
@prefix rdf:     <http://www.w3.org/1999/02/22-rdf-syntax-ns#> .
@prefix rdfs:    <http://www.w3.org/2000/01/rdf-schema#> .
@prefix skos:    <http://www.w3.org/2004/02/skos/core#> .
@prefix time:    <http://www.w3.org/2006/time#> .
@prefix vann:    <http://purl.org/vocab/vann/> .
@prefix vs:      <http://www.w3.org/2003/06/sw-vocab-status/ns#> .
@prefix wot:     <http://xmlns.com/wot/0.1/> .
@prefix xsd:     <http://www.w3.org/2001/XMLSchema#> .

ac:homepage
    a owl:ObjectProperty;
    rdfs:isDefinedBy ac:;
    rdfs:label "homepage";
    rdfs:comment "Links an audio resource to a corresponding web page" ;
    rdfs:subPropertyOf foaf:isPrimaryTopicOf;
# The domain ac:AudioManifestation is too strict in respect with sub-property
# mo:homepage, whose domain is owl:unionOf (mo:MusicalWork mo:MusicArtist
# mo:MusicalExpression mo:MusicalManifestation mo:MusicalItem).
# Maybe is better to use directly foaf:isPrimaryTopicOf or foaf:homepage?
#
#    rdfs:domain ac:AudioManifestation;
    rdfs:range foaf:Document.
mo:homepage rdfs:subPropertyOf ac:homepage.

ac:image
    a owl:ObjectProperty;
    rdfs:isDefinedBy ac:;
    rdfs:label "image";
    rdfs:comment """
        Indicates a pictorial image (JPEG, GIF, PNG, Etc.) of an audio resource.""";
    rdfs:subPropertyOf foaf:depiction;
# The domain ac:AudioManifestation is too strict in respect with sub-property
# mo:image, whose domain is owl:unionOf (mo:MusicalWork mo:MusicArtist
# mo:MusicalExpression mo:MusicalManifestation mo:MusicalItem).
# Maybe is better to use directly foaf:depiction?
#
#    rdfs:domain ac:AudioManifestation;
    rdfs:range foaf:Image.
mo:image rdfs:subPropertyOf ac:image.

# Is this the best way to represent authorship in this model?
ac:compiled
    a owl:ObjectProperty;
    rdfs:isDefinedBy ac:;
    rdfs:label "compiler";
    rdfs:comment """
        Used to relate a person or a group of people who created/compiled an
        audio manifestation." ;
    rdfs:domain foaf:Agent;
    rdfs:range ac:AudioManifestation.
mo:compiled rdfs:subPropertyOf ac:compiled.

ac:published
    a owl:ObjectProperty;
    rdfs:isDefinedBy ac:;
    rdfs:label "published";
    rdfs:comment """
        Used to relate a person or a group of people who published an audio
        manifestation." ;
    rdfs:domain foaf:Agent;
    rdfs:range ac:AudioManifestation.
mo:published rdfs:subPropertyOf ac:published.

ac:AudioClip
    a owl:Class;
    rdfs:isDefinedBy ac:;
    rdfs:label "Audio clip";
    rdfs:subClassOf ac:AudioManifestation.
mo:Track rdfs:subClassOf ac:AudioClip.

ac:duration
    a owl:DatatypeProperty;
    rdfs:isDefinedBy ac:;
    rdfs:label "duration in ms";
    rdfs:subPropertyOf mo:duration;
    rdfs:domain ac:AudioClip;
    rdfs:range xsd:int.
